# A small ontology to hold various scores for DCAT Resources
# such as FAIR and CARE scores
PREFIX dcat: <http://www.w3.org/ns/dcat#>
PREFIX dcterms: <http://purl.org/dc/terms/>
PREFIX owl: <http://www.w3.org/2002/07/owl#>
PREFIX qb: <http://purl.org/linked-data/cube#>
PREFIX rdfs: <http://www.w3.org/2000/01/rdf-schema#>
PREFIX scores: <https://linked.data.gov.au/def/scores/>
PREFIX sdmxm: <http://purl.org/linked-data/sdmx/2009/measure#>
PREFIX sdo: <https://schema.org/>
PREFIX skos: <http://www.w3.org/2004/02/skos/core#>
PREFIX time: <http://www.w3.org/2006/time#>
PREFIX xsd: <http://www.w3.org/2001/XMLSchema#>


<https://linked.data.gov.au/def/scores>
    a owl:Ontology ;
    skos:prefLabel "Scores Ontology"@en ;
    skos:definition "This is an ontology designed to represent the scores that have been calculated for catalogues resources according to various principles, such as the CARE and FAIR principles. The ontology also provides properties to link Resources to scores."@en ;
    sdo:dateCreated "2022-10-11"^^xsd:date ;
    sdo:dateModified "2022-10-11"^^xsd:date ;
    sdo:dateIssued "2022-10-11"^^xsd:date ;
    sdo:creator <https://orcid.org/0000-0002-8742-7730> ;
    sdo:publisher <https://linked.data.gov.au/org/idn> ;
    dcterms:provenance "This ontology was developed as part of the Indigenous Data Network's Catalogue Profile (https://linked.data.gov.au/def/idncp) in 2022. The structures of the various Scores - FAIR, CARE etc. - reflect those principles' structures." ;
    sdo:license "https://creativecommons.org/licenses/by/4.0/"^^xsd:anyURI ;
    owl:versionIRI <https://linked.data.gov.au/def/scores/0.0.1> ;
    owl:versionInfo "0.0.1" ;
    sdo:codeRespository "https://github.com/idn-au/idn-catalogue-profile/"^^xsd:anyURI ;
    sdo:copyrightHolder <https://linked.data.gov.au/org/idn> ;
    sdo:copyrightNotice "(c) Indigenous Data Network, 2022" ;
    sdo:copyrightYear "2022"^^xsd:gYear ;
.

<https://linked.data.gov.au/org/idn>
    a sdo:Organization ;
    sdo:name "Indigenous Data Network" ;
    sdo:description "The IDN is within the University of Melbourne. It was established in 2018 to support and coordinate the governance of Indigenous data for Aboriginal and Torres Strait Islander peoples and empower Aboriginal and Torres Strait Islander communities to decide their own local data priorities." ;
    sdo:url "https://mspgh.unimelb.edu.au/centres-institutes/centre-for-health-equity/research-group/indigenous-data-network"^^xsd:anyURI ;
.

<https://orcid.org/0000-0002-8742-7730>
    a sdo:Person ;
    sdo:name "Nicholas J. Car"@en ;
    sdo:email "nick@kurrawong.net"^^xsd:anyURI ;
.

scores:Score
    a owl:Class ;
    rdfs:subClassOf qb:ObservationGroup ;
    skos:prefLabel "Score"@en ;
    skos:definition "A Score is a value, or set of values, for a catalogues Resource that has been calculated from metadata or data elements known for the resource in accordance with a scoring principles or metric system, such as the FAIR principles"@en ;
    rdfs:isDefinedBy <https://linked.data.gov.au/def/scores> ;
    skos:example """
        <http://example.com/resource/x>
            a dcat:Resource ;
            scores:hasScore <http://example.com/score/y> ;
        .

        <http://example.com/score/y>
            a scores:Score ;
        .
        """ ;
    dcterms:provenance "Invented for this ontology" ;
.

scores:CareScore
    a owl:Class ;
    skos:prefLabel "CARE Score"@en ;
    skos:definition "A score according to the CARE Principles for Indigenous Data Governance (CARE: https://www.gida-global.org/care) principles"@en ;
    rdfs:isDefinedBy <https://linked.data.gov.au/def/scores> ;
    skos:example """
        <http://example.com/resource/x>
            a dcat:Resource ;
            scores:hasScore <http://example.com/score/y> ;
        .

        <http://example.com/score/y>
            a scores:CareScore ;
        .
        """ ;
    dcterms:source "https://ardc.edu.au/resource/the-care-principles/"^^xsd:anyURI ;
.

scores:FairScore
    a owl:Class ;
    skos:prefLabel "FAIR Score"@en ;
    skos:definition "A score according to the Findable, Accessible, Interoperable and Reusable (FAIR: https://www.go-fair.org/fair-principles/) principles"@en ;
    rdfs:isDefinedBy <https://linked.data.gov.au/def/scores> ;
    skos:example """
        <http://example.com/resource/x>
            a dcat:Resource ;
            scores:hasScore <http://example.com/score/y> ;
        .

        <http://example.com/score/y>
            a scores:FairScore ;
        .
        """ ;
    dcterms:source "https://force11.org/info/the-fair-data-principles/"^^xsd:anyURI ;
.

scores:LcLabelsScore
    a owl:Class ;
    skos:prefLabel "Local Context Labels Score"@en ;
    skos:definition "A score according to the Local Context Labels (LC Labels: https://localcontexts.org/)"@en ;
    rdfs:isDefinedBy <https://linked.data.gov.au/def/scores> ;
    skos:example """
        <http://example.com/resource/x>
            a dcat:Resource ;
            scores:hasScore <http://example.com/score/y> ;
        .

        <http://example.com/score/y>
            a scores:LcLabelsScore ;
        .
        """ ;
    dcterms:source "https://localcontexts.org/"^^xsd:anyURI ;
.

scores:hasScore
    a owl:ObjectProperty ;
    rdfs:subPropertyOf dcterms:relation ;
    rdfs:domain dcat:Resource ;
    rdfs:range scores:Score ;
    skos:prefLabel "has score"@en ;
    skos:definition "The subject Resource has a Score calculated for it from its metadata"@en ;
    rdfs:isDefinedBy <https://linked.data.gov.au/def/scores> ;
    skos:example """
        <http://example.com/resource/x>
            a dcat:Resource ;
            scores:hasScore <http://example.com/score/y> ;
        .

        <http://example.com/score/y>
            a scores:Score ;
        .
        """ ;
    skos:scopeNote "As per Data Cube modelling, a Score, being a group of Observations, a qb:ObservationGroup, is linked to the thing that is scored (observed), the catalogues Resource, via a property of the Observation instance. This property then is an alternate linking mechanism and not the only one or even the primary one: it is Resource-centric, as opposed to Observations-centric."@en ;
    dcterms:provenance "Invented for this ontology" ;
.

scores:refResource
    a qb:DimensionProperty ;
    rdfs:range dcat:Resource ;
    skos:prefLabel "Reference Resource"@en ;
    skos:definition "The catalogued Resource that the Score is for"@en ;
.

scores:refTime
    a qb:DimensionProperty ;
    rdfs:subPropertyOf time:hasTime ;
    rdfs:range time:TemporalEntity ;
    skos:prefLabel "Reference Time"@en ;
    skos:definition "The Temporal Entity that the Score is for"@en ;
.

scores:scoreValue
    a qb:MeasureProperty ;
    rdfs:subPropertyOf
        sdmxm:obsValue ,
        owl:DatatypeProperty ;
    skos:prefLabel "score value"@en ;
    skos:definition "The value of a dimension of a Score"@en ;
.

scores:fairScoreValue
    a qb:MeasureProperty ;
    rdfs:subPropertyOf scores:scoreValue ;
    rdfs:range xsd:positiveInteger ;
    skos:prefLabel "FAIR score value"@en ;
    skos:definition "The value of a dimension of a FAIR Score, i.e. F, A, I or R. FAIR scores are always positive integers."@en ;
.

# incomplete: no range
scores:careScoreValue
    a qb:MeasureProperty ;
    rdfs:subPropertyOf scores:scoreValue ;
    skos:prefLabel "CARE score value"@en ;
    skos:definition "The value of a dimension of a CARE Score, i.e. C, A, I or R."@en ;
.

scores:fairFScore
    a qb:MeasureProperty ;
    rdfs:subPropertyOf scores:fairScoreValue ;
    skos:prefLabel "Findability Score"@en ;
    dcterms:source "https://force11.org/info/the-fair-data-principles/"^^xsd:anyURI ;
.

scores:fairAScore
    a qb:MeasureProperty ;
    rdfs:subPropertyOf scores:fairScoreValue ;
    rdfs:range xsd:positiveInteger ;
    skos:prefLabel "Accessibility Score"@en ;
    dcterms:source "https://force11.org/info/the-fair-data-principles/"^^xsd:anyURI ;
.

scores:fairIScore
    a qb:MeasureProperty ;
    rdfs:subPropertyOf scores:fairScoreValue ;
    rdfs:range xsd:positiveInteger ;
    skos:prefLabel "Interoperability Score"@en ;
    dcterms:source "https://force11.org/info/the-fair-data-principles/"^^xsd:anyURI ;
.

scores:fairRScore
    a qb:MeasureProperty ;
    rdfs:subPropertyOf scores:fairScoreValue ;
    rdfs:range xsd:positiveInteger ;
    skos:prefLabel "Reusability Score"@en ;
    dcterms:source "https://force11.org/info/the-fair-data-principles/"^^xsd:anyURI ;
.
